Tests/FFI.lean
@@ -58,3 +58,17 @@ def arrays' : List ByteArray := [
 
 #lspec arrays'.zip arrays |>.foldl (init := .done) fun tSeq (x, y) =>
   tSeq ++ (test s!"{x} > {y}" $ x.ord y == .gt && x.ordC y == .gt)
+
+def sliceInputs : List (Nat × Nat) := [
+  (0, 0), (0, 1), (0, 2), (0, 3), (0, 4), (0, 5), (0, 6),
+  (1, 0), (1, 1), (1, 2), (1, 3), (1, 4), (1, 5), (1, 6),
+  (2, 0), (2, 1), (2, 2), (2, 3), (2, 4), (2, 5), (2, 6),
+  (3, 0), (3, 1), (3, 2), (3, 3), (3, 4), (3, 5), (3, 6),
+  (5, 0), (5, 1), (5, 2), (5, 3), (5, 4), (5, 5), (5, 6),
+  (6, 0), (6, 1), (6, 2), (6, 3), (6, 4), (6, 5), (6, 6)
+]
+
+#lspec arrays.foldl (init := .done) fun tSeq arr =>
+  sliceInputs.foldl (init := tSeq) fun tSeq (i, n) =>
+    tSeq ++ test s!"Lean/C match for {arr} sliced {i} {n}"
+      (arr.sliceL i n == arr.sliceC i n)
